generational/spec/GC.Gen.CheneyBFS.fst
@@ -63,6 +63,27 @@ let fwd_well_formed_covers_reachable
 
 #push-options "--z3rlimit 40 --fuel 1 --ifuel 0"
 
+/// Helper: cheney_forward_normal preserves forwarding entries
+private let cheney_forward_normal_fwd_monotone
+  (minor: minor_state) (cs: CheneySpec.cheney_state) (addr: U64.t) (x: U64.t)
+  : Lemma (requires cs.cs_fwd x <> 0UL)
+          (ensures (CheneySpec.cheney_forward_normal minor cs addr).cs_fwd x <> 0UL)
+  =
+  if cs.cs_fwd addr <> 0UL then
+    CheneySpec.cheney_forward_normal_noop minor cs addr
+  else if not (Seq.mem addr (minor_objects minor)) then
+    CheneySpec.cheney_forward_normal_noop minor cs addr
+  else if minor_wosize minor addr = 0 then
+    CheneySpec.cheney_forward_normal_noop_wz0 minor cs addr
+  else begin
+    let wz = minor_wosize minor addr in
+    let res = promote_object minor cs.cs_major addr cs.cs_fp wz in
+    if res.new_addr = 0UL then
+      CheneySpec.cheney_forward_normal_noop_oom minor cs addr
+    else
+      CheneySpec.cheney_forward_normal_success minor cs addr
+  end
+
 let forward_one_fwd_monotone
   (minor: minor_state) (cs: CheneySpec.cheney_state) (addr: U64.t) (x: U64.t)
   : Lemma (requires cs.cs_fwd x <> 0UL /\ minor_infix_wf minor)
@@ -71,24 +92,17 @@ let forward_one_fwd_monotone
   if cs.cs_fwd addr <> 0UL then
     CheneySpec.cheney_forward_one_noop minor cs addr
   else if is_infix_in_minor minor addr then begin
-    // Infix case: forward parent preserves fwd entries, extend_forwarding
-    // only touches addr (which is <> x since cs.cs_fwd addr = 0 but cs.cs_fwd x <> 0).
-    assume ((CheneySpec.cheney_forward_one minor cs addr).cs_fwd x <> 0UL)
+    // Infix case: for y <> addr, result's fwd y = cs'.fwd y where cs' = forward_normal parent.
+    // We know x <> addr (since cs.cs_fwd x <> 0 but cs.cs_fwd addr = 0).
+    // By normal monotone on parent, cs'.cs_fwd x <> 0.
+    // By infix_fwd lemma, result.cs_fwd x = cs'.cs_fwd x <> 0.
+    let parent = infix_parent minor addr in
+    cheney_forward_normal_fwd_monotone minor cs parent x;
+    CheneySpec.cheney_forward_one_infix_fwd minor cs addr x
   end
   else begin
     CheneySpec.cheney_forward_one_normal minor cs addr;
-    if not (Seq.mem addr (minor_objects minor)) then
-      CheneySpec.cheney_forward_normal_noop minor cs addr
-    else if minor_wosize minor addr = 0 then
-      CheneySpec.cheney_forward_normal_noop_wz0 minor cs addr
-    else begin
-      let wz = minor_wosize minor addr in
-      let res = promote_object minor cs.cs_major addr cs.cs_fp wz in
-      if res.new_addr = 0UL then
-        CheneySpec.cheney_forward_normal_noop_oom minor cs addr
-      else
-        CheneySpec.cheney_forward_normal_success minor cs addr
-    end
+    cheney_forward_normal_fwd_monotone minor cs addr x
   end
 
 #pop-options
